src/Cancel.v
@@ -1,0 +1,232 @@
+From Coq Require List.
+
+From Tactical Require Import Misc.
+
+Require Import SepLogic.Reification.Varmap.
+Require Import SepLogic.Reification.Sorting.
+Require Import SepLogic.Mem.
+Require Export SepLogic.Pred.
+
+Import PredNotations.
+Local Open Scope pred.
+
+Set Implicit Arguments.
+
+(*! Setting up reified syntax *)
+Instance pred_def A V : Default (pred A V) := @emp A V.
+
+Section Mem.
+  Context (A V:Type).
+  Notation pred := (pred A V).
+  Notation emp := (@emp A V).
+
+  (* non-recursive part of reification *)
+  Inductive op_element :=
+  | Leaf (x:pred)
+  | Atom (i:varmap.I)
+  | LiftedProp (P:Prop)
+  | ConstEmp
+  .
+
+  Definition interpret_e (vm: varmap.t pred) (e: op_element) : pred :=
+    match e with
+    | Leaf x => x
+    | Atom i => varmap.find i vm
+    | LiftedProp P => lift P
+    | ConstEmp => emp
+    end.
+
+  Inductive op_tree :=
+  | Element (e: op_element)
+  | StarNode (l r: op_tree)
+  .
+
+
+  Fixpoint interpret (vm: varmap.t pred) t : pred :=
+    match t with
+    | Element e => interpret_e vm e
+    | StarNode l r => star (interpret vm l) (interpret vm r)
+    end.
+End Mem.
+
+(*! Boilerplate for doing reification *)
+Ltac reify_helper A V term ctx :=
+  let reify_rec term ctx := reify_helper A V term ctx in
+  lazymatch ctx with
+  | context[varmap.cons ?i term _] =>
+    constr:( (ctx, Element (Atom A V i)) )
+  | _ =>
+    lazymatch term with
+    | @emp _ _ => constr:( (ctx, Element (ConstEmp A V)) )
+    | lift ?P => constr:( (ctx, Element (LiftedProp A V P)) )
+    | star ?x ?y =>
+      let ctx_x := reify_rec x ctx in
+      let ctx_y := reify_rec y (fst ctx_x) in
+      let r := (eval cbv [fst snd] in
+                   (fst ctx_y, @StarNode A V (snd ctx_x) (snd ctx_y))) in
+      constr:(r)
+    | _ =>
+      let v' := (eval cbv [varmap.length] in (varmap.length ctx)) in
+      let ctx' := constr:( varmap.cons v' term ctx ) in
+      constr:( (ctx', Element (Atom A V v')) )
+    end
+  end.
+
+Ltac quote_with A V ctx term :=
+  let ctx_x := reify_helper A V term ctx in
+  let ctx := (eval cbv [fst] in (fst ctx_x)) in
+  let x := (eval cbv [snd] in (snd ctx_x)) in
+  constr:(interpret ctx x).
+
+Ltac quote term rx :=
+  match type of term with
+  | pred ?A ?V =>
+    let reified := quote_with A V (varmap.empty (pred A V)) term in
+    rx reified
+  end.
+
+Ltac quote_impl :=
+  match goal with
+  | |- @pimpl ?A ?V ?x ?y =>
+    quote x ltac:(fun x' =>
+                    match x' with
+                    | interpret ?ctx ?xt =>
+                      let y' := quote_with A V ctx y in
+                      match y' with
+                      | interpret ?ctx' ?yt =>
+                        change (interpret ctx' xt ===> interpret ctx' yt)
+                      end
+                    end)
+  end.
+
+Notation "[ i1 |-> v1 ]  :: vm" := (varmap.cons i1 v1 vm)
+                                     (at level 20, vm at level 80,
+                                      only printing).
+Notation "[]" := (varmap.empty _) (at level 0, only printing).
+
+Theorem reify_test A V (p1 p2 p3: pred A V) :
+  p1 * p2 * p3 ===> p1 * (p2 * p3).
+Proof.
+  quote_impl.
+Abort.
+
+(*! Proving theorems on reified syntax *)
+Section Mem.
+  Context (A V:Type).
+  Notation pred := (pred A V).
+  Notation emp := (@emp A V).
+
+  Notation op_tree := (op_tree A V).
+  Notation op_element := (op_element A V).
+
+  Import List.ListNotations.
+  Local Open Scope list.
+
+  Fixpoint flatten (t:op_tree) : list op_element :=
+    match t with
+    | Element e => match e with
+                  | ConstEmp _ _ => []
+                  | _ => [e]
+                  end
+    | StarNode l r => flatten l ++ flatten r
+    end.
+
+  (*
+  Fixpoint flatten (t:op_tree) : list Prop * list op_element :=
+    match t with
+    | Element e => match e with
+                  | ConstEmp _ _ => ([], [])
+                  | LiftedProp _ _ P => ([P], [])
+                  | _ => ([], [e])
+                  end
+    | StarNode l r => let (ps1, es1) := flatten l in
+                     let (ps2, es2) := flatten r in
+                     (ps1 ++ ps2, es2 ++ es2)
+    end.
+   *)
+
+  Fixpoint int_l vm (l: list op_element) : pred :=
+    match l with
+    | [] => emp
+    | e::es => star (interpret_e vm e) (int_l vm es)
+    end.
+
+  Hint Resolve (ltac:(reflexivity) : forall (p:pred), p === p).
+
+  Theorem int_l_app vm l1 l2 :
+    int_l vm (l1 ++ l2) === int_l vm l1 * int_l vm l2.
+  Proof.
+    induction l1; simpl.
+    rewrite star_emp_l; auto.
+    rewrite <- star_assoc.
+    rewrite IHl1; auto.
+  Qed.
+
+  Fixpoint flatten_props (l: list Prop) : Prop :=
+    match l with
+    | [] => True
+    | [P] => P
+    | P::Ps => P /\ flatten_props Ps
+    end.
+
+  Theorem interpret_flatten vm t :
+      interpret vm t === int_l vm (flatten t).
+  Proof.
+    induction t; simpl.
+    destruct e; simpl;
+      try rewrite star_emp_r; auto.
+    rewrite int_l_app.
+    rewrite IHt1, IHt2; auto.
+  Qed.
+
+  Theorem int_l_perm vm l1 l2:
+      Permutation l1 l2 ->
+      int_l vm l1 === int_l vm l2.
+  Proof.
+    induction 1; simpl; auto.
+    - rewrite IHPermutation; auto.
+    - rewrite ?star_assoc.
+      apply star_respects_iff; auto.
+      rewrite star_comm; auto.
+    - rewrite IHPermutation1, IHPermutation2; auto.
+  Qed.
+
+  Definition get_key (e:op_element) : option nat :=
+    match e with
+    | Atom _ _ i => Some (S i)
+    | LiftedProp _ _ _ => Some 0
+    | _ => None
+    end.
+
+  Theorem int_l_sort vm l :
+      int_l vm l === int_l vm (sortBy get_key l).
+  Proof.
+    apply int_l_perm.
+    apply sortBy_permutation.
+  Qed.
+
+  Theorem int_l_sort_eqn vm l1 l2 :
+      int_l vm (sortBy get_key l1) === int_l vm (sortBy get_key l2) ->
+      int_l vm l1 === int_l vm l2.
+  Proof.
+    intros.
+    rewrite <- ?int_l_sort in H; auto.
+  Qed.
+
+  Theorem int_l_sort_impl vm l1 l2 :
+      int_l vm (sortBy get_key l1) ===> int_l vm (sortBy get_key l2) ->
+      int_l vm l1 ===> int_l vm l2.
+  Proof.
+    intros.
+    setoid_rewrite <- int_l_sort in H; auto.
+  Qed.
+
+End Mem.
+
+Ltac norm :=
+  intros;
+  quote_impl;
+  rewrite ?interpret_flatten;
+  apply int_l_sort_impl;
+  simpl;
+  repeat (apply impl_with_lift; intros).
