src/CancelTests.v
@@ -1,0 +1,47 @@
+Require Import SepLogic.Cancel.
+
+Import PredNotations.
+Local Open Scope pred.
+
+Section Tests.
+  Context (A V:Type).
+  Notation pred := (pred A V).
+  Implicit Types (p:pred).
+  Implicit Types (P Q:Prop).
+
+  Theorem test_assoc p1 p2 p3 :
+    p1 * p2 * p3 ===> p1 * (p2 * p3).
+  Proof.
+    norm; reflexivity.
+  Qed.
+
+  Theorem test_reorder p1 p2 p3 :
+    p1 * p2 * p3 ===> p1 * (p3 * p2).
+  Proof.
+    norm; reflexivity.
+  Qed.
+
+  Theorem test_collapse_emp p1 :
+    emp * p1 ===> p1 * emp * emp.
+  Proof.
+    norm; reflexivity.
+  Qed.
+
+  Theorem test_lift_prop p1 p2 p3 Q :
+    p1 * p2 * p3 * [Q] ===> p1 * (p3 * p2).
+  Proof.
+    norm.
+    match goal with
+    | [ H: Q |- _ ] => reflexivity
+    end.
+  Qed.
+
+  Theorem test_norm_repeat p1 p2 :
+    p1 * p2 ===> p2 * p1.
+  Proof.
+    norm.
+    try (progress norm; fail 1 "norm should do nothing if repeated").
+    reflexivity.
+  Qed.
+
+End Tests.
